Replace Natural with Nat in names

naturals/CommutingCanonicalNatImpl.v
@@ -1,48 +1,48 @@
 Require Import CanonicalNatImpl CommutingNatIntf.
 
-(* An implementation of CommutingNaturalInterface using the definitions in
- * CanonicalNaturalImpl. Of course, all of the commutativity properties hold
+(* An implementation of CommutingNatInterface using the definitions in
+ * CanonicalNat. Of course, all of the commutativity properties hold
  * trivially *)
-Module CommutingCanonicalNaturalImpl <: CommutingNaturalInterface.
-  Definition N := CanonicalNaturalImpl.N.
-  Definition zero := CanonicalNaturalImpl.zero.
-  Definition succ := CanonicalNaturalImpl.succ.
-  Definition pred := CanonicalNaturalImpl.pred.
-  Definition add := CanonicalNaturalImpl.add.
-  Definition sub := CanonicalNaturalImpl.sub.
-  Definition comp := CanonicalNaturalImpl.comp.
+Module CommutingCanonicalNat <: CommutingNatInterface.
+  Definition N := CanonicalNat.N.
+  Definition zero := CanonicalNat.zero.
+  Definition succ := CanonicalNat.succ.
+  Definition pred := CanonicalNat.pred.
+  Definition add := CanonicalNat.add.
+  Definition sub := CanonicalNat.sub.
+  Definition comp := CanonicalNat.comp.
 
   Definition convert (n:N) := n.
   Lemma convert_injective : forall n n' : N, convert n = convert n' -> n = n'.
     auto.
   Defined.
 
-  Lemma zero_commutes : convert zero = CanonicalNaturalImpl.zero.
+  Lemma zero_commutes : convert zero = CanonicalNat.zero.
     auto.
   Defined.
 
   Lemma succ_commutes : forall n : N,
-      convert (succ n) = CanonicalNaturalImpl.succ (convert n).
+      convert (succ n) = CanonicalNat.succ (convert n).
     auto.
   Defined.
 
   Lemma pred_commutes : forall n : N,
-      convert (pred n) = CanonicalNaturalImpl.pred (convert n).
+      convert (pred n) = CanonicalNat.pred (convert n).
     auto.
   Defined.
 
   Lemma add_commutes : forall n n' : N,
-      convert (add n n') = CanonicalNaturalImpl.add (convert n) (convert n').
+      convert (add n n') = CanonicalNat.add (convert n) (convert n').
     auto.
   Defined.
 
   Lemma sub_commutes : forall n n' : N,
-      convert (sub n n') = CanonicalNaturalImpl.sub (convert n) (convert n').
+      convert (sub n n') = CanonicalNat.sub (convert n) (convert n').
     auto.
   Defined.
 
   Lemma comp_commutes : forall n n' : N,
-      comp n n' = CanonicalNaturalImpl.comp (convert n) (convert n').
+      comp n n' = CanonicalNat.comp (convert n) (convert n').
     auto.
   Defined.
-End CommutingCanonicalNaturalImpl.
+End CommutingCanonicalNat.
