naturals/CommutingNatIntf.v
@@ -1,8 +1,8 @@
 Require Import NatIntf CanonicalNatImpl.
 
-(* An extension of NaturalInterface for implementations that commute with
- * CanonicalNatImpl *)
-Module Type CommutingNaturalInterface <: NaturalInterface.
+(* An extension of NatInterface for implementations that commute with
+ * CanonicalNat *)
+Module Type CommutingNatInterface <: NatInterface.
   Parameter N : Type.
 
   Parameter zero : N.
@@ -12,21 +12,21 @@ Module Type CommutingNaturalInterface <: NaturalInterface.
   Parameter sub : N -> N -> N.
   Parameter comp : N -> N -> comparison.
 
-  Parameter convert : N -> CanonicalNaturalImpl.N.
+  Parameter convert : N -> CanonicalNat.N.
 
   (* We require convert to be injective, because it makes a lot of subsequent
    * proofs a lot simpler. This requirement is not necessary, however. *)
   Axiom convert_injective : forall n n' : N, convert n = convert n' -> n = n'.
 
-  Axiom zero_commutes : convert zero = CanonicalNaturalImpl.zero.
+  Axiom zero_commutes : convert zero = CanonicalNat.zero.
   Axiom succ_commutes : forall n : N,
-    convert (succ n) = CanonicalNaturalImpl.succ (convert n).
+    convert (succ n) = CanonicalNat.succ (convert n).
   Axiom pred_commutes : forall n : N,
-    convert (pred n) = CanonicalNaturalImpl.pred (convert n).
+    convert (pred n) = CanonicalNat.pred (convert n).
   Axiom add_commutes : forall n n' : N,
-    convert (add n n') = CanonicalNaturalImpl.add (convert n) (convert n').
+    convert (add n n') = CanonicalNat.add (convert n) (convert n').
   Axiom sub_commutes : forall n n' : N,
-    convert (sub n n') = CanonicalNaturalImpl.sub (convert n) (convert n').
+    convert (sub n n') = CanonicalNat.sub (convert n) (convert n').
   Axiom comp_commutes : forall n n' : N,
-    comp n n' = CanonicalNaturalImpl.comp (convert n) (convert n').
-End CommutingNaturalInterface.
+    comp n n' = CanonicalNat.comp (convert n) (convert n').
+End CommutingNatInterface.
